lib/steel/pulse/Pulse.Checker.ExtractFrame.fst
@@ -1,0 +1,701 @@
+module Pulse.Checker.ExtractFrame
+
+module T = FStar.Tactics.V2
+module RT = FStar.Reflection.Typing
+
+open FStar.List.Tot
+open Pulse.Syntax
+open Pulse.Typing
+open Pulse.Checker.Pure
+open Pulse.Checker.Common
+open Pulse.Checker.Comp
+open Pulse.Syntax.Printer
+
+open FStar.Reflection.V2.TermEq
+
+open FStar.Printf
+
+module FV = Pulse.Typing.FV
+module MT = Pulse.Typing.Metatheory
+
+open FStar.Algebra.CommMonoid.Equiv
+open FStar.Squash
+
+#push-options "--admit_smt_queries true"
+
+// TODO: Move printing stuff to printer?
+// START PRINTING
+
+let print_term (t: term): T.Tac unit
+  = T.print (term_to_string t)
+
+let rec print_list_terms' (l: list term): T.Tac unit
+= match l with
+| [] -> T.print "]"
+| t::q -> (T.print ", "; print_term t; print_list_terms' q)
+
+let print_list_terms (l: list term): T.Tac unit
+  = match l with
+  | [] -> T.print "[]"
+  | t::q -> (T.print "["; print_term t; print_list_terms' q)
+
+let indent (level:string) = level ^ " "
+
+let st_equiv_to_string (#g: env) #c1 #c2 (level: string) (eq: st_equiv g c1 c2)
+  : T.Tac string
+  = (*if comp_pre c1 = comp_pre c2 && comp_post c1 = comp_post c2
+    then T.print "Trivial equivalence!"
+    else T.print "Somehow non-trivial equivalence...";*)
+    sprintf "st_equiv\n%s pre1: %s\n%s pre2: %s\n%s post1: %s\n%s post2: %s"
+  //pre: (%s) (%s)) (post: (%s) (%s))"
+  level
+  (term_to_string (comp_pre c1))
+  level
+  (term_to_string (comp_pre c2))
+  level
+  (term_to_string (comp_post c1))
+  level
+  (term_to_string (comp_post c2))
+
+#push-options "--z3rlimit 10"
+let rec st_typing_to_string' (#g:env) (#t:st_term) (#c:comp) (level: string) (ty: st_typing g t c)
+//let rec st_typing_to_string (ty: st_typing)
+  : T.Tac string
+  = match ty with
+    | T_Abs g x q b u body c _ _ -> "T_Abs"
+    | T_STApp g head _ q res arg _ _ -> "T_STapp"
+    | T_Return g c use_eq u t e post x _ _ _ -> "T_Return"
+    | T_Lift g e c1 c2 _ _ -> "T_Lift"
+    | T_Bind g e1 e2 c1 c2 b _ c ty1 _ ty2 _ ->
+      sprintf "T_Bind \n (%s); \n (%s)"
+      (st_typing_to_string' (indent level) ty1)
+      (st_typing_to_string' (indent level) ty2)
+    | T_TotBind g e1 e2 t1 c2 x _ ty' ->
+      sprintf "T_TotBind (%s)"
+      (st_typing_to_string' (indent level) ty')
+    | T_Frame g e c frame _ ty' ->
+      sprintf "T_Frame (frame=%s) (\n%s%s)"
+      (term_to_string frame)
+      level
+      (st_typing_to_string' (indent level) ty')
+    | T_Equiv g e c c' ty' equiv ->
+      sprintf "T_Equiv (%s) (\n%s%s)"
+      //(st_equiv_to_string level equiv)
+      "..."
+      level
+      (st_typing_to_string' (indent level) ty')
+    | T_Par g eL cL eR cR x _ _ ty1 ty2 -> "T_Par"
+    | _ -> "Unsupported"
+    // TODO: If
+#pop-options
+
+let st_typing_to_string (#g:env) (#t:st_term) (#c:comp) (ty: st_typing g t c)
+  = st_typing_to_string' #g #t #c "" ty
+//let st_typing_to_string #g #t #c (ty: st_typing g t c) = st_typing_to_string' "" ty
+
+// END PRINTING
+
+
+
+open Pulse.Checker.VPropEquiv
+
+// Would need a stronger postcondition
+// Like pre and post are equiv
+// needs typing for one of the two pres...
+let create_st_equiv
+  (g: env)
+  (c: comp_st)
+  (c': comp_st{st_equiv_pre c c'})
+  (equiv_pre: vprop_equiv g (comp_pre c) (comp_pre c'))
+  //(typing_pre: either (tot_typing g (comp_pre c) tm_vprop) (tot_typing g (comp_pre c') tm_vprop))
+  (typing_pre: tot_typing g (comp_pre c) tm_vprop)
+  (typing_res: tot_typing g (comp_res c) (tm_type (comp_u c)))
+  //(x:var{fresh....})
+  //(equiv_post: x:var -> vprop_equiv g (comp_post c) (comp_post c'))
+: st_equiv g c c'
+= let x = fresh g in
+  assume ( ~(x `Set.mem` freevars (comp_post c)) /\
+          ~(x `Set.mem` freevars (comp_post c')) );
+  //assume (st_equiv_pre c c');
+  (*
+  let tot1: Ghost.erased (tot_typing g (comp_pre c) tm_vprop) = (
+    match typing_pre with
+    | Inl ty -> ty
+    | Inr ty -> (vprop_equiv_typing equiv_pre)._2 ty
+  ) in
+  *)
+  let tot3: Ghost.erased (tot_typing (push_binding g x ppname_default (comp_res c)) (open_term (comp_post c) x) tm_vprop) = magic() in
+  let equiv_post: Ghost.erased (vprop_equiv (push_binding g x ppname_default (comp_res c)) (open_term (comp_post c) x) (open_term (comp_post c') x)) = magic() in
+  ST_VPropEquiv g c c' x typing_pre typing_res tot3 equiv_pre equiv_post
+
+// TODO:
+let inv_typing_comp_res #g #e (#c: comp{stateful_comp c}) (ty: st_typing g e c):
+  tot_typing g (comp_res c) (tm_type (comp_u c))
+= admit()
+
+let inv_typing_comp_pre #g #e (#c: comp{stateful_comp c}) (ty: st_typing g e c):
+  tot_typing g (comp_pre c) tm_vprop
+= admit()
+
+// This function replaces T_Frame with empty frames by T_Equiv
+// Do we actually need to prove equivalence?
+let rec replace_frame_emp_with_equiv #g #t #c (ty: st_typing g t c):
+  Tot (st_typing g t c) (decreases ty)
+  = match ty with
+  | T_Frame g e c' frame tot_ty ty' -> 
+  // comp_pre c = comp_pre_pre (add_frame c')
+  if Tm_Emp? frame.t then
+    let pre = comp_pre c' in
+    let eq1: vprop_equiv g (tm_star frame pre) pre = VE_Unit g pre in
+    let eq2: vprop_equiv g (tm_star pre frame) (tm_star frame pre) = VE_Comm g pre frame in
+    let eq3: vprop_equiv g (tm_star pre frame) pre = VE_Trans g _ _ _ eq2 eq1 in
+    let eq_pre: vprop_equiv g (comp_pre c') (tm_star (comp_pre c') frame) = VE_Sym g _ _ eq3 in
+    let typing_res: tot_typing g (comp_res c) (tm_type (comp_u c)) = inv_typing_comp_res ty' in
+    let st_eq: st_equiv g c' c = create_st_equiv g c' c eq_pre (inv_typing_comp_pre ty') typing_res in
+      T_Equiv g e c' c (replace_frame_emp_with_equiv ty') st_eq
+  else ty
+  | T_Equiv g e c c' ty' equiv ->
+  T_Equiv g e c c' (replace_frame_emp_with_equiv ty') equiv
+  | T_Bind g e1 e2 c1 c2 b x c ty1 tot1 ty2 tot2 ->
+  T_Bind g e1 e2 c1 c2 b x c (replace_frame_emp_with_equiv ty1) tot1 (replace_frame_emp_with_equiv ty2) tot2
+  | _ -> ty
+
+let rec collect_frames #g #e #c (ty: st_typing g e c):
+  T.Tac ((l:list term{length l > 0}) & tot_typing g (hd l) tm_vprop)
+= match ty with
+  | T_Frame g e c' frame tot_ty ty' -> (| [frame], tot_ty |)
+  | T_Equiv g e c c' ty' equiv -> collect_frames ty'
+  | T_Bind g e1 e2 c1 c2 b x c ty1 _ ty2 _ -> 
+  let (| l1, tot1 |) = collect_frames ty1 in
+  let (| l2, _ |) = collect_frames ty2 in
+  (| l1 @ l2, tot1 |)
+  | _ -> T.fail "Unable to figure out frame at this leaf"
+ 
+(*
+let deq (a: host_term) (b: host_term): (r:bool{r <==> (a == b)}) =
+  (assume (faithful a); assume (faithful b); term_eq_dec a b)
+
+let delta (a: host_term) (b: host_term): nat
+  = if deq a b then 1 else 0
+  *)
+
+(*
+TODO:
+let rec countt (l: seqterm) (x: host_term): nat
+  = match l with
+  | [] -> 0
+  | t::q -> delta t x + countt q x
+  *)
+
+//let single (#a: Type) (x: a): seq a = create 1 x
+
+//let prepend (#a: Type) (t: a) (q: seq a) = Seq.append (single t) q
+
+//let atom = (t:term{~(Tm_Star? t.t) /\ ~(Tm_Emp? t.t)})
+let atom = term
+
+let typed_list_atoms g = list (x:atom & tot_typing g x tm_vprop)
+// is destructive
+let rec compute_intersection_aux g (ft: atom) (ty: tot_typing g ft tm_vprop) (l: list atom):
+  Tot (typed_list_atoms g & list atom)
+  (decreases (length l))
+  = match l with
+  | [] -> ([], [])
+  | t::q -> if eq_tm t ft then ([(| ft, ty |) ], q)
+  else let (a, b) = compute_intersection_aux g ft ty q in (a, t::b)
+  (*
+  if Seq.length l = 0 then (Seq.empty, Seq.empty)
+  else (let (t, q) = (head l, tail l) in
+    if deq ft t then (Seq.create 1 ft, q)
+    else let (a, b) = compute_intersection_aux ft q in (a, prepend t b)
+  *)
+  (*
+  // how to link
+  // delta t x = countt l x - countt b x
+  *)
+
+// spec
+(*
+let rec countt_compute_intersection (ft: host_term) (l: seqterm) (x: host_term):
+  Lemma (let (a, b) = compute_intersection_aux ft l in (countt l x = countt a x + countt b x
+  /\ length a <= 1 /\ length l = length a + length b
+  /\ countt a x <= 1
+  /\ (~(deq ft x) ==> countt a x = 0)
+  /\ (countt a x = 1 <==> (deq ft x /\ countt l x >= 1))
+  ))
+= match l with
+  | [] -> ()
+  | t::q -> if deq ft t then ()
+  else countt_compute_intersection ft q x
+  *)
+
+// Could be improved (in terms of performance) if we had an order on host_terms
+let rec compute_intersection g (l1: typed_list_atoms g) (l2: list atom):
+  Tot (typed_list_atoms g) (decreases (length l1))
+ = match l1 with
+  | [] -> []
+  | t::q -> let (a, b) = compute_intersection_aux g t._1 t._2 l2 // l2 = a @ b
+  in a @ compute_intersection g q b
+ (*
+  if length l1 = 0 then Seq.empty
+  else (let (t, q) = (head l1, tail l1) in
+    let (a, b) = compute_intersection_aux t l2 // l2 = a @ b
+    in append a (compute_intersection q b)
+  )
+  *)
+
+(*
+let rec countt_append (l1: seqterm) (l2: seqterm) (x: host_term):
+  Lemma (countt (l1 @ l2) x = countt l1 x + countt l2 x)
+  = match l1 with
+  | [] -> ()
+  | t::q -> countt_append q l2 x
+
+let rec compute_intersection_included (l1: seqterm) (l2: seqterm) (x: host_term):
+  Lemma (let l = compute_intersection l1 l2 in
+  countt l x = min (countt l1 x) (countt l2 x))
+= match l1 with
+  | [] -> ()
+  | t::q -> let (a, b) = compute_intersection_aux t l2 in
+   countt_compute_intersection t l2 x;
+  calc (=) {
+    countt (compute_intersection l1 l2) x;
+    = { countt_append a (compute_intersection q b) x }
+    countt a x + countt (compute_intersection q b) x;
+    = { compute_intersection_included q b x }
+    countt l2 x - countt b x + min (countt q x) (countt b x);
+    = {}
+    min (countt q x - countt b x + countt l2 x) (countt l2 x);
+    = {}
+    min (countt l1 x) (countt l2 x);
+  }
+  *)
+
+
+(*
+let add_range t = with_range (Tm_FStar t) (Range.range_0)
+
+let from_list_to_term (g: env) (l: seqterm): term
+  = let l' = map_seq add_range l in
+  FStar.Seq.Permutation.foldm_snoc (vprop_monoid g) l'
+  //tm_star tm_emp l'
+
+//let term_to_list_inv
+// Not correct...
+
+let from_list_to_term_single g ft
+: Lemma (vprop_equiv g (from_list_to_term g (single ft)) (add_range ft))
+= 
+  map_seq_create add_range 1 ft;
+  Seq.Permutation.foldm_snoc_singleton (vprop_monoid g) (add_range ft)
+
+(*assert (index (single ft) 0 == ft)
+  map_seq_create add_range 1 ft;
+  assert (map_seq add_range (single ft) == single (add_range ft))
+  //map_seq_index add_range (single ft) 0
+  *)
+
+
+
+// collects a subset of all host terms
+// should collect typing proofs as well
+let rec term_to_list (t: term): seqterm
+  = match t.t with
+  | Tm_FStar ft -> single ft
+  | Tm_Star l r -> append (term_to_list l) (term_to_list r)
+  | _ -> admit() //T.fail "Could not convert the term to a list"
+  *)
+
+//let vprop_as_list_atom (t: vprop): (list atom)
+//  = (assume false; vprop_as_list t)
+
+let rec vprop_as_list_typed #g (vp:term) (ty: tot_typing g vp tm_vprop)
+  : typed_list_atoms g// list (x:atom & tot_typing g x tm_vprop)
+  = match vp.t with
+    | Tm_Emp -> []
+    | Tm_Star vp0 vp1 ->
+    vprop_as_list_typed vp0 (star_typing_inversion_l #g #vp0 #vp1 ty)
+    @ vprop_as_list_typed vp1 (star_typing_inversion_r #g #vp0 #vp1 ty)
+    | _ -> [(| vp, ty|)]
+
+//let rec compute_intersection g (l1: typed_list_atoms g) (l2: list atom):
+//  Tot (typed_list_atoms g) (decreases (length l1))
+
+let compute_intersection_list g (l: list term{length l > 0}) (ty: tot_typing g (hd l) tm_vprop):
+  T.Tac (list (x:atom & tot_typing g x tm_vprop))
+  = match l with
+  | [] -> []
+  | t::q -> fold_left (compute_intersection g) (vprop_as_list_typed t ty) (map vprop_as_list q)
+
+let rec list_of_FStar_term_to_string l: T.Tac string
+= match l with
+  | [] -> ""
+  | t::q -> T.term_to_string t ^ ", " ^ list_of_FStar_term_to_string q
+
+(*
+let rec remove_host_term_from_term (ht: host_term) (t: term): bool & term
+// returns (b, t')
+// b means we have removed it successfully, and t' is t minus ht
+// b false implies t = t'
+  = match t.t with
+  | Tm_FStar ft -> if deq ft ht then (assert (ht == ft); (true, with_range Tm_Emp t.range)) else (false, t)
+  | Tm_Star l r -> let (b, l') = remove_host_term_from_term ht l in
+  if b then (true, with_range (Tm_Star l' r) t.range)
+  else let (b', r') = remove_host_term_from_term ht r in
+    if b' then (true, with_range (Tm_Star l r') t.range) else (false, t)
+  | _ -> (false, t)
+// should return true in every "good" call
+
+let rec remove_from_vprop (l: seqterm) (t: term):
+  T.Tac term
+  // need to prove that it's equiv...
+= if length l = 0 then t
+  else let (ht, q) = (head l, tail l) in remove_from_vprop q ((remove_host_term_from_term ht t)._2)
+(*match l with
+  | [] -> t
+  | ht::q -> remove_from_vprop q ((remove_host_term_from_term ht t)._2)
+  *)
+  *)
+
+(*
+let rec remove_from_vprop_equiv g (l: seqterm) (t: term):
+  T.Tac (vprop_equiv g t (tm_star (from_list_to_term g l) (remove_from_vprop l t)))
+= admit()
+*)
+
+//let star_with_range r a b = with_range (Tm_Star a b) r
+
+
+let ve_unit_rev (g: env) (t:term): vprop_equiv g (tm_star t tm_emp) t
+  = let eq1: vprop_equiv g (tm_star tm_emp t) t = VE_Unit _ t in
+  let eq2: vprop_equiv g (tm_star t tm_emp) (tm_star tm_emp t)
+  = VE_Comm _ _ _ in
+  VE_Trans _ _ _ _ eq2 eq1
+
+  // need to show that appending is OK?
+  (*
+let append_from_list_to_term_equiv (g: env) (l1 l2: seqterm):
+  Lemma (vprop_equiv g
+    (from_list_to_term g (append l1 l2))
+    (tm_star (from_list_to_term g l1) (from_list_to_term g l2))
+    )
+= FStar.Seq.Permutation.foldm_snoc_append (vprop_monoid g) (map_seq add_range l1) (map_seq add_range l2);
+  map_seq_append add_range l1 l2;
+  ()
+  *)
+
+// if there 
+//let unsquash_test (#p: Type) (s: squash p): GTot p
+//  = admit()
+
+(*
+let rec term_to_list_vprop_equiv (g: env) (t: term):
+  T.Tac (vprop_equiv g t (from_list_to_term g (term_to_list t)))
+= match t.t with
+  | Tm_FStar ft -> VE_Sym g _ _ (elim_squash (from_list_to_term_single g ft))
+  | Tm_Star l r -> 
+  let eql = term_to_list_vprop_equiv g l in
+  let eqr = term_to_list_vprop_equiv g r in
+  let ll = term_to_list l in
+  let rr = term_to_list r in
+  let eqlr: vprop_equiv g (tm_star l r) (tm_star (from_list_to_term g ll) (from_list_to_term g rr))
+  = VE_Ctxt g _ _ _ _ eql eqr in
+  append_from_list_to_term_equiv g ll rr;
+  let eq_append: vprop_equiv g
+    (tm_star (from_list_to_term g ll) (from_list_to_term g rr))
+    (from_list_to_term g (append ll rr))
+   = VE_Sym _ _ _ (elim_squash ()) in
+  //let sq: squash (vprop_equiv g (from_list_to_term g (append ll rr)) (from_list_to_term g (term_to_list t))) = () in
+  //let eq_append: vprop_equiv g _ (from_list_to_term g (term_to_list t)) = VE_Sym _ _ _ sq in
+  VE_Trans g _ _ _ eqlr eq_append
+  | _ -> fail g None "Could not convert term to an equivalent list representation"
+*)
+
+open Pulse.Checker.Framing
+
+let remove_from_vprop #g (#ctxt: term) (inter: term) (ctxt_typing: tot_typing g ctxt tm_vprop):
+  T.Tac
+  (res:term & tot_typing g res tm_vprop & vprop_equiv g (tm_star inter res) ctxt)
+= match check_frameable ctxt_typing inter with
+| Inl x -> x
+| Inr _ -> fail g None "Failure to remove intersection from frame..."
+
+let rec extract_common_frame #g #t #c #inter
+  (inter_typed: Ghost.erased (tot_typing g inter tm_vprop)) (ty: st_typing g t c):
+  T.Tac (st_typing g t c) (decreases ty)
+  = match ty with
+  | T_Frame g e c0 frame tot_ty ty' ->
+  let (| f1, tot_ty1, eq_21_f |) = remove_from_vprop inter tot_ty in
+  let c1 = add_frame c0 f1 in
+  let f2 = inter in
+  let eq_12_f: vprop_equiv g (tm_star f1 f2) frame = VE_Trans _ _ _ _ (VE_Comm _ f1 f2) eq_21_f in
+  let eqf12: vprop_equiv g frame (tm_star f1 f2) = VE_Sym _ _ _ eq_12_f in
+  let c2 = add_frame c1 f2 in
+  let tot_ty2: Ghost.erased (tot_typing g f2 tm_vprop) = inter_typed in
+  let ty1 = T_Frame g e c0 f1 tot_ty1 ty' in
+  let ty2 = T_Frame g e c1 f2 tot_ty2 ty1 in
+  let pre = comp_pre c0 in
+  let eq': vprop_equiv g (tm_star pre (tm_star f1 f2)) (tm_star pre frame) =
+    VE_Ctxt g _ _ _ _ (VE_Refl g pre) (VE_Sym g _ _ eqf12) in
+  let eq_assoc: vprop_equiv g (tm_star (tm_star pre f1) f2) (tm_star pre (tm_star f1 f2))
+    = VE_Sym _ _ _ (VE_Assoc _ _ _ _) in
+  let needed_eq: vprop_equiv g (tm_star (tm_star pre f1) f2) (tm_star pre frame) =
+    VE_Trans _ _ _ _ eq_assoc eq'
+  in
+  let typing_pre_c0: tot_typing g (comp_pre c0) tm_vprop = inv_typing_comp_pre ty' in
+  let typing_pre_c1: tot_typing g (comp_pre c1) tm_vprop = star_typing #g #(comp_pre c0) #f1 typing_pre_c0 tot_ty1 in
+  let typing_pre_c2: tot_typing g (comp_pre c2) tm_vprop = star_typing #g #(comp_pre c1) #f2 typing_pre_c1 inter_typed in
+  let typing_res: tot_typing g (comp_res c2) (tm_type (comp_u c2)) = inv_typing_comp_res ty' in
+  let st_eq: st_equiv g c2 c = create_st_equiv g c2 c needed_eq typing_pre_c2 typing_res in
+  T_Equiv g e c2 c ty2 st_eq
+  // replace frame by frame-common, and put that into common frame
+  // and an equiv
+  // Example: frame = A * B * C
+  // Common: B
+  // Result:
+  // Equiv (A * B * C) ((A * C) * B)
+  // {
+  //    Frame B (Frame (A * C) ... )
+  // }
+  | T_Equiv g e c c' ty' equiv ->
+  T_Equiv g e c c' (extract_common_frame inter_typed ty') equiv
+  | T_Bind g e1 e2 c1 c2 b x c ty1 tot1 ty2 tot2 ->
+  assert (fresh_wrt x g Set.empty);
+  let ntyped: Ghost.erased (tot_typing _ inter tm_vprop)
+    = Pulse.Typing.Metatheory.tot_typing_weakening x (comp_res c1) inter_typed in
+  T_Bind g e1 e2 c1 c2 b x c (extract_common_frame inter_typed ty1) tot1 (extract_common_frame #_ #_ #_ #inter ntyped ty2) tot2
+  | _ -> fail g None "No common frame to extract..." // bad, should not happen
+
+
+#pop-options
+//#push-options "--admit_smt_queries true"
+#push-options "--z3rlimit 20"
+
+//#set-options "--split_queries always --query_stats"
+
+
+let bring_frame_top_bind_aux #g #t1 #c1 #t2 #c2
+(b:binder { b.binder_ty == comp_res c1 })
+(x: var{None? (lookup g x)  /\ ~(x `Set.mem` freevars_st t2) })
+(ty1:st_typing g t1 c1{T_Frame? ty1})
+(ty2:st_typing (push_binding g x ppname_default (comp_res c1)) (open_st_term_nv t2 (b.binder_ppname, x)) c2{T_Frame? ty2})
+//(bcomp: bind_comp g x c1 c2 c)
+: T.Tac (c': comp & st_typing g (wr (Tm_Bind { binder=b; head=t1; body=t2 })) c')
+=
+admit()
+(*
+match ty1 with
+| T_Frame _ _ c1'' f1 totf1 ty1' -> (
+    let ty1': st_typing g e1 c1'' = ty1' in
+  match ty2 with
+  | T_Frame _ _ c2'' f2 totf2 ty2' ->
+    let g2 = push_binding g x ppname_default (comp_res c1') in
+    let ty2': st_typing g2 _ c2'' = ty2' in
+    let b':(b':binder{Mkbinder?.binder_ty b' == comp_res c1'}) =
+      {
+        binder_ty = comp_res c1'; binder_ppname = b.binder_ppname
+      } in
+    (
+      assume (bind_comp_compatible c1' c2');
+      assume (f1 == f2);
+      assume (bind_comp_pre x c1'' c2'');
+      let c': comp_st = bind_comp_out c1'' c2'' in
+      let tot_ty1: Ghost.erased (tot_typing g (comp_res c1') (tm_type (comp_u c1'))) = inv_typing_comp_res ty1 in
+      let bcomp': bind_comp g x c1'' c2'' c' = Bind_comp g x c1'' c2'' (magic()) (magic()) (magic()) in
+      //let (| e, c', ty' |)
+      //= Pulse.Typing.Combinators.mk_bind g (comp_pre c1'') e1 e2 c1'' c2'' (Pulse.Syntax.Base.v_as_nv x) ty1' tot_ty1 ty2' (magic()) (magic())
+      //in
+      //let ty': st_typing _ _ _ = bound._1 in
+      let ty': st_typing _ _ _ = T_Bind g e1 e2 c1'' c2'' b' x c' ty1' tot_ty1 ty2' bcomp' in
+      let e: st_term = {range = e1.range; term = Tm_Bind {binder=b; head=e1; body=e2}} in
+      let c'': comp_st = add_frame c' f1 in
+      let ty'': st_typing g _ c'' = T_Frame g e c' f1 totf1 ty' in
+      let jeq: vprop_equiv g (comp_pre c'') (comp_pre c1) =
+        VE_Trans _ _ _ _ (VE_Refl _ _) (ST_VPropEquiv?.equiv_pre eq1) in
+      let typing_res: tot_typing g (comp_res c'') (tm_type (comp_u c'')) = inv_typing_comp_res ty'' in
+      let typing_pre: tot_typing g (comp_pre c'') tm_vprop = inv_typing_comp_pre ty'' in
+      let eq: st_equiv g c'' c = create_st_equiv g c'' c jeq typing_pre typing_res in
+      Mkdtuple3 c'' ty'' eq)
+  | _ -> fail g None "Unexpected issue while bringing the frame to the top"
+)
+// | _ -> fail g None "Unexpected issue while bringing the frame to the top"
+*)
+
+
+#pop-options
+
+let st_typing_frame g t c = (ty:st_typing g t c{T_Frame? ty})
+
+(*
+this thing should be preserved
+let bind_comp_compatible (c1 c2:comp_st)
+  : prop
+  = match c1, c2 with
+    | C_STGhost inames1 _, C_STGhost inames2 _ -> inames1 == inames2
+    | C_ST _, C_ST _ -> True
+    | _, _ -> False
+*)
+
+let comp_same (c1 c2: comp)
+  = match c1, c2 with
+  | C_ST _, C_ST _ -> true
+  | C_STAtomic _ _, C_STAtomic _ _ -> true
+  | C_STGhost _ _, C_STGhost _ _ -> true
+  | C_Tot _, C_Tot _ -> true
+  | _ -> false
+
+let bring_frame_top_bind #g #t1 #c1 #t2 (#c2: comp_st{bind_comp_compatible c1 c2})
+(x: var{None? (lookup g x)  /\ ~(x `Set.mem` freevars_st t2) })
+(b:binder { b.binder_ty == comp_res c1 })
+(ty1: st_typing_frame g t1 c1{T_Frame? ty1})
+(ty2: st_typing_frame (push_binding g x ppname_default (comp_res c1)) (open_st_term_nv t2 (b.binder_ppname, x)) c2)
+//(ty1:st_typing g t1 c1{T_Frame? ty1})
+//(ty2:st_typing (push_binding g x ppname_default (comp_res c1)) (open_st_term_nv t2 (b.binder_ppname, x)) c2{T_Frame? ty2})
+//(bcomp: bind_comp g x c1 c2 c)
+: T.Tac (
+  c': comp{ comp_res c' == comp_res c2 /\ comp_same c' c2 }
+  & (st_typing_frame g (wr (Tm_Bind { binder=b; head=t1; body=t2 })) c'))
+=
+match ty1 with
+| T_Frame _ _ c1' f1 totf1 ty1' -> (
+    let ty1': st_typing g t1 c1' = ty1' in
+    match ty2 with
+    | T_Frame _ _ c2' f2 totf2 ty2' ->
+      let gx = push_binding g x ppname_default (comp_res c1) in
+      let t2x = open_st_term_nv t2 (b.binder_ppname, x) in
+      //let g2 = push_binding g x ppname_default (comp_res c1') in
+      let ty2': st_typing gx t2x c2' = ty2' in
+      assume (bind_comp_compatible c1' c2');
+      let c': comp_st = bind_comp_out c1' c2' in
+      let typing_res: tot_typing g (comp_res c1') (tm_type (comp_u c1')) = magic() in
+      let bcomp: bind_comp g x c1' c2' c' = magic() in
+      let ty_bind = T_Bind g t1 t2 c1' c2' b x c' ty1' typing_res ty2' bcomp in
+      let t: st_term = {range = t1.range; term = Tm_Bind {binder=b; head=t1; body=t2}} in
+      let c'': comp_st = add_frame c' f1 in
+      let ty_frame: st_typing g _ c'' = T_Frame g t c' f1 totf1 ty_bind in
+      (| c'', ty_frame |)
+    | _ -> fail g None "Should not happen"
+)
+| _ -> fail g None "Should not happen"
+
+let bind_comp_compatible_add_frame (c: comp_st) f:
+  Lemma (bind_comp_compatible (add_frame c f) c)
+= admit()
+
+#push-options "--z3rlimit 20"
+// Up to equivalence...
+let rec bring_frame_top #g #t #c (ty: st_typing g t c):
+// should allow to change the computation, as long as it's equivalent
+// we put back the equiv at the end? Not really needed
+  //T.Tac (c': comp & st_typing g t c' & st_equiv g c' c) //(decreases ty)
+  T.Tac (
+    c': comp{ comp_res c' == comp_res c /\ comp_same c c'
+    /\ ((stateful_comp c /\ stateful_comp c') ==> bind_comp_compatible c c') } // /\ (not (C_Tot? c) ==> bind_comp_compatible c c') } 
+    & st_typing_frame g t c') //(decreases ty)
+  =
+  match ty with
+  | T_Frame g e c0 frame tot_ty ty' ->
+    bind_comp_compatible_add_frame c0 frame;
+    (| c, ty |) // frame at the top: we're done
+  | T_Equiv _ _ _ _ ty1 _ -> bring_frame_top ty1
+  | T_Bind _ t1 t2 c1 c2 b x c' ty1 _ ty2 bcomp2 ->
+    (
+      let (| c1', ty1' |) = bring_frame_top ty1 in
+      let c1': comp_st = c1' in
+      let ty1': st_typing g t1 c1' = ty1' in
+      let (| c2', ty2' |) = bring_frame_top ty2 in
+      let c2': comp_st = c2' in
+      let gx = push_binding g x ppname_default (comp_res c1) in
+      assume (bind_comp_compatible c1' c2');
+      (*
+     let bind_comp_compatible (c1 c2:comp_st)
+  : prop
+  = match c1, c2 with
+    | C_STGhost inames1 _, C_STGhost inames2 _ -> inames1 == inames2
+    | C_ST _, C_ST _ -> True
+    | _, _ -> False
+      *)
+      let ty2': st_typing gx (open_st_term_nv t2 (b.binder_ppname, x)) c2' = ty2' in
+      let (| c', ty' |) = bring_frame_top_bind x b ty1' ty2' in
+      let ty': st_typing_frame g (wr (Tm_Bind {binder=b; head=t1; body=t2})) c' = ty' in
+      let ty': st_typing_frame g t c' = ty' in
+      assume (stateful_comp c /\ stateful_comp c' ==> bind_comp_compatible c c');
+      (| c', ty' |)
+    )
+  | _ -> fail g None "No frame to bring to the top..." // bad, should not happen
+
+let get_typing_deriv_and_frame #g #t #c (ty: st_typing g t c):
+  T.Tac (c':comp & st_typing g t c' & vprop) (decreases ty)
+= let (| c', ty' |) = bring_frame_top ty in
+  (
+    match ty' with
+    | T_Frame _ _ c'' f tot ty' -> (| c'', ty',  f |)
+    | _ -> fail g None "Did not find a frame at the top..."
+  )
+
+let rec list_as_vprop_typed g (l: list (a: atom & tot_typing g a tm_vprop)):
+  t:term & tot_typing g t tm_vprop
+= match l with
+| [] -> (| tm_emp, emp_typing #g |)
+| (| t, ty |) :: q -> 
+let (| qt, qty |) = list_as_vprop_typed g q in
+(| tm_star t qt, star_typing ty qty |)
+
+let compute_frame (#g: env)
+  (#t: st_term)
+  (#c: comp)
+  (ty: st_typing g t c)
+: T.Tac (frame: vprop & tot_typing g frame tm_vprop)
+=
+  // removing empty frames
+  let ty = replace_frame_emp_with_equiv ty in
+  // collecting all frames
+  let (| frames, typing_frame |) = collect_frames ty in
+  // computing the meet of all frames
+  let inter_list = compute_intersection_list g frames typing_frame in
+  //let (| frame, frame_typed |) =
+  list_as_vprop_typed g inter_list
+
+let extract_frame #g #t #c #frame
+  (typing_frame: tot_typing g frame tm_vprop) (ty: st_typing g t c)
+= get_typing_deriv_and_frame (extract_common_frame typing_frame ty)
+
+// Without retypechecking
+let compute_and_extract_frame (#g: env) (#t: st_term) (#c: comp)
+  (ty: st_typing g t c)
+: T.Tac (frame:vprop & tot_typing g frame tm_vprop & c': comp & st_typing g t c')
+=
+  let (| frame, frame_typed |) = compute_frame ty in
+  let (| c', typing, _|) = extract_frame frame_typed ty in
+  (| frame, frame_typed, c', typing |)
+
+#push-options "--query_stats --z3rlimit 10"
+// For the moment: Using the double typechecking
+let infer_frame_and_typecheck (#g: env) (#ctxt: term)
+  (allow_inst: bool)
+  (t: st_term)
+  (ctxt_typing: tot_typing g ctxt tm_vprop)
+  (post_hint: post_hint_opt g)
+  (check':bool -> check_t)
+  (modify_type_derivation: bool)
+: T.Tac (
+  t: st_term &
+  c:comp{(stateful_comp c /\ ~modify_type_derivation) ==> comp_post_matches_hint c post_hint} &
+  frame:vprop &
+  tot_typing g frame tm_vprop &
+  (st_typing g t c &
+  (squash (stateful_comp c /\ ~modify_type_derivation) -> vprop_equiv g (tm_star frame (comp_pre c)) ctxt))
+ )
+=
+  // checking in the large context
+  let (| t, c, big_typing |) = check' allow_inst g t ctxt ctxt_typing None in
+  // computing the frame
+  let (| frame, frame_typed |) = compute_frame big_typing in
+  if modify_type_derivation then
+    let (| c, typing, _ |) = extract_frame frame_typed big_typing in
+    (| t, c, frame, frame_typed, (typing, (fun _ -> VE_Refl g frame)) |)
+  else
+    // approach 1: we now retypecheck in `ctxt - frame`
+    let (| inferred_pre, typing_pre, equiv_pre |) = remove_from_vprop frame ctxt_typing in
+    let (| t, c, typing |) = check' allow_inst g t inferred_pre typing_pre post_hint in
+    (| t, c, frame, frame_typed, (typing, (fun _ -> equiv_pre)) |)
