lib/steel/pulse/Pulse.Checker.ExtractFrame.fsti
@@ -1,0 +1,45 @@
+module Pulse.Checker.ExtractFrame
+
+module T = FStar.Tactics.V2
+
+open Pulse.Syntax
+open Pulse.Typing
+open Pulse.Checker.Common
+
+// Simple wrapper around check_frameable
+val remove_from_vprop (#g: env) (#ctxt: term)
+  (to_remove: term) (ctxt_typing: tot_typing g ctxt tm_vprop):
+  T.Tac (res:term & tot_typing g res tm_vprop & vprop_equiv g (tm_star to_remove res) ctxt)
+
+// computes a frame that works for the whole typing derivation
+val compute_frame (#g: env) (#t: st_term) (#c: comp)
+  (ty: st_typing g t c)
+: T.Tac (frame: vprop & tot_typing g frame tm_vprop)
+
+// removes a frame from a typing derivation
+// this frame must be included in all non-trivial frame applications
+// in the typing derivation
+val extract_frame (#g: env) (#t: st_term) (#c: comp) (#frame: vprop)
+  (typing_frame: tot_typing g frame tm_vprop) (ty: st_typing g t c)
+: T.Tac (c':comp & st_typing g t c' & vprop)
+
+// composes compute_frame with extract_frame
+val compute_and_extract_frame (#g: env) (#t: st_term) (#c: comp)
+  (ty: st_typing g t c)
+: T.Tac (frame:vprop & tot_typing g frame tm_vprop & c': comp & st_typing g t c')
+
+val infer_frame_and_typecheck (#g: env) (#ctxt: term)
+  (allow_inst: bool)
+  (t: st_term)
+  (ctxt_typing: tot_typing g ctxt tm_vprop)
+  (post_hint: post_hint_opt g)
+  (check':bool -> check_t)
+  (modify_type_derivation: bool)
+: T.Tac (
+  t: st_term &
+  c:comp{(stateful_comp c /\ ~modify_type_derivation) ==> comp_post_matches_hint c post_hint} &
+  frame:vprop &
+  tot_typing g frame tm_vprop &
+  (st_typing g t c &
+  (squash (stateful_comp c /\ ~modify_type_derivation) -> vprop_equiv g (tm_star frame (comp_pre c)) ctxt))
+ )
